src/coq/Handlers/MemoryModules/FiniteSizeof.v
@@ -83,36 +83,18 @@ Module FinSizeof : Sizeof.
     lia.
   Qed.
 
-  Lemma sizeof_dtyp_packed_struct_0 :
-    sizeof_dtyp (DTYPE_Packed_struct nil) = 0%N.
+  (* Should take padding into account *)
+  Lemma sizeof_dtyp_Struct :
+    forall dts,
+      sizeof_dtyp (DTYPE_Struct dts) = List.fold_left (fun acc dt => N.add acc (sizeof_dtyp dt)) dts 0%N.
   Proof.
     reflexivity.
   Qed.
-
-  Lemma sizeof_dtyp_packed_struct_cons :
-    forall dt dts,
-      sizeof_dtyp (DTYPE_Packed_struct (dt :: dts)) = (sizeof_dtyp dt + sizeof_dtyp (DTYPE_Packed_struct dts))%N.
+    
+  Lemma sizeof_dtyp_Packed_struct :
+    forall dts,
+      sizeof_dtyp (DTYPE_Packed_struct dts) = List.fold_left (fun acc dt => N.add acc (sizeof_dtyp dt)) dts 0%N.
   Proof.
-    intros dt dts.
-    cbn.
-    rewrite fold_sum_acc.
-    reflexivity.
-  Qed.
-
-  Lemma sizeof_dtyp_struct_0 :
-    sizeof_dtyp (DTYPE_Struct nil) = 0%N.
-  Proof.
-    reflexivity.
-  Qed.
-
-  (* TODO: this should take padding into account *)
-  Lemma sizeof_dtyp_struct_cons :
-    forall dt dts,
-      sizeof_dtyp (DTYPE_Struct (dt :: dts)) = (sizeof_dtyp dt + sizeof_dtyp (DTYPE_Struct dts))%N.
-  Proof.
-    intros dt dts.
-    cbn.
-    rewrite fold_sum_acc.
     reflexivity.
   Qed.
 
@@ -138,7 +120,7 @@ Module FinSizeof : Sizeof.
 End FinSizeof.
 
 Inductive UByte (uvalue : Type) :=
-| mkUByte (uv : uvalue) (dt : dtyp) (idx : uvalue) (sid : store_id) : UByte uvalue.
+| mkUByte (uv : uvalue) (dt : dtyp) (idx : N) (sid : store_id) : UByte uvalue.
 
 Module FinByte (ADDR : MemoryAddress.ADDRESS) (IP : MemoryAddress.INTPTR) (SIZEOF : Sizeof) (LLVMEvents:LLVM_INTERACTIONS(ADDR)(IP)(SIZEOF)) : ByteImpl(ADDR)(IP)(SIZEOF)(LLVMEvents)
 with  Definition SByte := UByte LLVMEvents.DV.uvalue
