src/coq/Semantics/DynamicValues.v
@@ -386,7 +386,7 @@ Module DVALUE(A:Vellvm.Semantics.MemoryAddress.ADDRESS)(IP:Vellvm.Semantics.Memo
   (* Extract the `idx` byte from a uvalue `uv`, which was stored with
    type `dt`. `idx` 0 is the least significant byte. `sid` is the "store
    id". *)
-  | UVALUE_ExtractByte      (uv : uvalue) (dt : dtyp) (idx : uvalue) (sid : store_id)
+  | UVALUE_ExtractByte      (uv : uvalue) (dt : dtyp) (idx : N) (sid : store_id)
   | UVALUE_ConcatBytes      (uvs : list uvalue) (dt : dtyp)
   .
   Set Elimination Schemes.
@@ -431,7 +431,7 @@ Module DVALUE(A:Vellvm.Semantics.MemoryAddress.ADDRESS)(IP:Vellvm.Semantics.Memo
     | UVALUE_Select cnd v1 v2 =>
         S (uvalue_measure cnd + uvalue_measure v1 + uvalue_measure v2)
     | UVALUE_ExtractByte uv dt idx sid =>
-        S (uvalue_measure uv + uvalue_measure idx)
+        S (uvalue_measure uv)
     | UVALUE_ConcatBytes uvs dt =>
         S (list_sum (map uvalue_measure uvs))
     end.
@@ -525,7 +525,7 @@ Module DVALUE(A:Vellvm.Semantics.MemoryAddress.ADDRESS)(IP:Vellvm.Semantics.Memo
     Hypothesis IH_ExtractValue   : forall (t:dtyp) (vec:uvalue) (idxs:list LLVMAst.int), P vec -> P (UVALUE_ExtractValue t vec idxs).
     Hypothesis IH_InsertValue    : forall (t:dtyp) (vec:uvalue) (et:dtyp) (elt:uvalue) (idxs:list LLVMAst.int), P vec -> P elt -> P (UVALUE_InsertValue t vec et elt idxs).
     Hypothesis IH_Select         : forall (cnd:uvalue) (v1:uvalue) (v2:uvalue), P cnd -> P v1 -> P v2 -> P (UVALUE_Select cnd v1 v2).
-    Hypothesis IH_ExtractByte : forall (uv : uvalue) (dt : dtyp) (idx : uvalue) (sid : N), P uv -> P idx -> P (UVALUE_ExtractByte uv dt idx sid).
+    Hypothesis IH_ExtractByte : forall (uv : uvalue) (dt : dtyp) (idx : N) (sid : N), P uv -> P (UVALUE_ExtractByte uv dt idx sid).
     Hypothesis IH_ConcatBytes : forall (dt : dtyp) (uvs : list uvalue),
         (forall u, In u uvs -> P u) ->
         P (UVALUE_ConcatBytes uvs dt).
@@ -609,7 +609,7 @@ Module DVALUE(A:Vellvm.Semantics.MemoryAddress.ADDRESS)(IP:Vellvm.Semantics.Memo
     Hypothesis IH_ExtractValue   : forall (t:dtyp) (vec:uvalue) (idxs:list LLVMAst.int), P vec -> P (UVALUE_ExtractValue t vec idxs).
     Hypothesis IH_InsertValue    : forall (t:dtyp) (vec:uvalue) (et:dtyp) (elt:uvalue) (idxs:list LLVMAst.int), P vec -> P elt -> P (UVALUE_InsertValue t vec et elt idxs).
     Hypothesis IH_Select         : forall (cnd:uvalue) (v1:uvalue) (v2:uvalue), P cnd -> P v1 -> P v2 -> P (UVALUE_Select cnd v1 v2).
-    Hypothesis IH_ExtractByte : forall (uv : uvalue) (dt : dtyp) (idx : uvalue) (sid : N), P uv -> P idx -> P (UVALUE_ExtractByte uv dt idx sid).
+    Hypothesis IH_ExtractByte : forall (uv : uvalue) (dt : dtyp) (idx : N) (sid : N), P uv -> P (UVALUE_ExtractByte uv dt idx sid).
     Hypothesis IH_ConcatBytes : forall (dt : dtyp) (uvs : list uvalue),
         (forall u, InT u uvs -> P u) ->
         P (UVALUE_ConcatBytes uvs dt).
@@ -663,181 +663,6 @@ Module DVALUE(A:Vellvm.Semantics.MemoryAddress.ADDRESS)(IP:Vellvm.Semantics.Memo
     Qed.
   End UvalueRec.
 
-  Section UvalueInd'.
-    Variable P : uvalue -> Prop.
-    Hypothesis IH_Addr           : forall a, P (UVALUE_Addr a).
-    Hypothesis IH_I1             : forall x, P (UVALUE_I1 x).
-    Hypothesis IH_I8             : forall x, P (UVALUE_I8 x).
-    Hypothesis IH_I32            : forall x, P (UVALUE_I32 x).
-    Hypothesis IH_I64            : forall x, P (UVALUE_I64 x).
-    Hypothesis IH_IPTR            : forall x, P (UVALUE_IPTR x).
-    Hypothesis IH_Double         : forall x, P (UVALUE_Double x).
-    Hypothesis IH_Float          : forall x, P (UVALUE_Float x).
-    Hypothesis IH_Undef          : forall t, P (UVALUE_Undef t).
-    Hypothesis IH_Poison         : forall t, P (UVALUE_Poison t).
-    Hypothesis IH_Oom            : forall t, P (UVALUE_Oom t).
-    Hypothesis IH_None           : P UVALUE_None.
-    Hypothesis IH_Struct_nil     : P (UVALUE_Struct []).
-    Hypothesis IH_Struct_cons    : forall uv uvs, P uv -> P (UVALUE_Struct uvs) -> P (UVALUE_Struct (uv :: uvs)).
-    Hypothesis IH_Packed_struct_nil     : P (UVALUE_Packed_struct []).
-    Hypothesis IH_Packed_struct_cons    : forall uv uvs, P uv -> P (UVALUE_Packed_struct uvs) -> P (UVALUE_Packed_struct (uv :: uvs)).
-    Hypothesis IH_Array_nil          : P (UVALUE_Array []).
-    Hypothesis IH_Array_cons          : forall uv uvs, P uv -> P (UVALUE_Array uvs) -> P (UVALUE_Array (uv :: uvs)).
-    Hypothesis IH_Vector_nil          : P (UVALUE_Vector []).
-    Hypothesis IH_Vector_cons          : forall uv uvs, P uv -> P (UVALUE_Vector uvs) -> P (UVALUE_Vector (uv :: uvs)).
-    Hypothesis IH_IBinop         : forall (iop:ibinop) (v1:uvalue) (v2:uvalue), P v1 -> P v2 -> P (UVALUE_IBinop iop v1 v2).
-    Hypothesis IH_ICmp           : forall (cmp:icmp)   (v1:uvalue) (v2:uvalue), P v1 -> P v2 -> P (UVALUE_ICmp cmp v1 v2).
-    Hypothesis IH_FBinop         : forall (fop:fbinop) (fm:list fast_math) (v1:uvalue) (v2:uvalue), P v1 -> P v2 -> P (UVALUE_FBinop fop fm v1 v2).
-    Hypothesis IH_FCmp           : forall (cmp:fcmp)   (v1:uvalue) (v2:uvalue), P v1 -> P v2 -> P (UVALUE_FCmp cmp v1 v2).
-    Hypothesis IH_Conversion     : forall (conv:conversion_type) (t_from:dtyp) (v:uvalue) (t_to:dtyp), P v -> P (UVALUE_Conversion conv t_from v t_to).
-    Hypothesis IH_GetElementPtr  : forall (t:dtyp) (ptrval:uvalue) (idxs:list (uvalue)), P ptrval -> (forall idx, In idx idxs -> P idx) -> P (UVALUE_GetElementPtr t ptrval idxs).
-    Hypothesis IH_ExtractElement : forall (t:dtyp) (vec: uvalue) (idx: uvalue), P vec -> P idx -> P (UVALUE_ExtractElement t vec idx).
-    Hypothesis IH_InsertElement  : forall (t:dtyp) (vec: uvalue) (elt:uvalue) (idx:uvalue), P vec -> P elt -> P idx -> P (UVALUE_InsertElement t vec elt idx).
-    Hypothesis IH_ShuffleVector  : forall (t:dtyp) (vec1:uvalue) (vec2:uvalue) (idxmask:uvalue), P vec1 -> P vec2 -> P idxmask -> P (UVALUE_ShuffleVector t vec1 vec2 idxmask).
-    Hypothesis IH_ExtractValue   : forall (t:dtyp) (vec:uvalue) (idxs:list LLVMAst.int), P vec -> P (UVALUE_ExtractValue t vec idxs).
-    Hypothesis IH_InsertValue    : forall (t:dtyp) (vec:uvalue) (et:dtyp) (elt:uvalue) (idxs:list LLVMAst.int), P vec -> P elt -> P (UVALUE_InsertValue t vec et elt idxs).
-    Hypothesis IH_Select         : forall (cnd:uvalue) (v1:uvalue) (v2:uvalue), P cnd -> P v1 -> P v2 -> P (UVALUE_Select cnd v1 v2).
-    Hypothesis IH_ExtractByte : forall (uv : uvalue) (dt : dtyp) (idx : uvalue) (sid : N), P uv -> P idx -> P (UVALUE_ExtractByte uv dt idx sid).
-    Hypothesis IH_ConcatBytes : forall (dt : dtyp) (uvs : list uvalue),
-        (forall u, In u uvs -> P u) ->
-        P (UVALUE_ConcatBytes uvs dt).
-
-    Lemma uvalue_ind' : forall (uv:uvalue), P uv.
-      fix IH 1.
-      remember P as P0 in IH.
-      destruct uv; auto; subst.
-      - revert fields.
-        fix IHfields 1. intros [|u' fields']. intros. apply IH_Struct_nil.
-        apply IH_Struct_cons.
-        apply IH.
-        apply IHfields.
-      - revert fields.
-        fix IHfields 1. intros [|u' fields']. intros. apply IH_Packed_struct_nil.
-        apply IH_Packed_struct_cons.
-        apply IH.
-        apply IHfields.
-      - revert elts.
-        fix IHelts 1. intros [|u elts']. intros. apply IH_Array_nil.
-        apply IH_Array_cons.
-        apply IH.
-        apply IHelts.
-      - revert elts.
-        fix IHelts 1. intros [|u elts']. intros. apply IH_Vector_nil.
-        apply IH_Vector_cons.
-        apply IH.
-        apply IHelts.
-      - apply IH_IBinop; auto.
-      - apply IH_ICmp; auto.
-      - apply IH_FBinop; auto.
-      - apply IH_FCmp; auto.
-      - apply IH_Conversion; auto.
-      - apply IH_GetElementPtr. apply IH.
-        { revert idxs.
-          fix IHidxs 1. intros [|u idxs']. intros. inversion H.
-          intros u' [<-|Hin]. apply IH. eapply IHidxs. apply Hin.
-        }
-      - apply IH_ExtractElement; auto.
-      - apply IH_InsertElement; auto.
-      - apply IH_ShuffleVector; auto.
-      - apply IH_ExtractValue; auto.
-      - apply IH_InsertValue; auto.
-      - apply IH_Select; auto.
-      - apply IH_ExtractByte; auto.
-      - apply IH_ConcatBytes.
-        { revert uvs.
-          fix IHuvs 1. intros [|u uvs']. intros. inversion H.
-          intros u' [<-|Hin]. apply IH. eapply IHuvs. apply Hin.
-        }
-    Qed.
-  End UvalueInd'.
-
-  Section UvalueRec'.
-    Variable P : uvalue -> Set.
-    Hypothesis IH_Addr           : forall a, P (UVALUE_Addr a).
-    Hypothesis IH_I1             : forall x, P (UVALUE_I1 x).
-    Hypothesis IH_I8             : forall x, P (UVALUE_I8 x).
-    Hypothesis IH_I32            : forall x, P (UVALUE_I32 x).
-    Hypothesis IH_I64            : forall x, P (UVALUE_I64 x).
-    Hypothesis IH_IPTR            : forall x, P (UVALUE_IPTR x).
-    Hypothesis IH_Double         : forall x, P (UVALUE_Double x).
-    Hypothesis IH_Float          : forall x, P (UVALUE_Float x).
-    Hypothesis IH_Undef          : forall t, P (UVALUE_Undef t).
-    Hypothesis IH_Poison         : forall t, P (UVALUE_Poison t).
-    Hypothesis IH_Oom            : forall t, P (UVALUE_Oom t).
-    Hypothesis IH_None           : P UVALUE_None.
-    Hypothesis IH_Struct_nil     : P (UVALUE_Struct []).
-    Hypothesis IH_Struct_cons    : forall uv uvs, P uv -> P (UVALUE_Struct uvs) -> P (UVALUE_Struct (uv :: uvs)).
-    Hypothesis IH_Packed_struct_nil     : P (UVALUE_Packed_struct []).
-    Hypothesis IH_Packed_struct_cons    : forall uv uvs, P uv -> P (UVALUE_Packed_struct uvs) -> P (UVALUE_Packed_struct (uv :: uvs)).
-    Hypothesis IH_Array_nil          : P (UVALUE_Array []).
-    Hypothesis IH_Array_cons          : forall uv uvs, P uv -> P (UVALUE_Array uvs) -> P (UVALUE_Array (uv :: uvs)).
-    Hypothesis IH_Vector_nil          : P (UVALUE_Vector []).
-    Hypothesis IH_Vector_cons          : forall uv uvs, P uv -> P (UVALUE_Vector uvs) -> P (UVALUE_Vector (uv :: uvs)).
-    Hypothesis IH_IBinop         : forall (iop:ibinop) (v1:uvalue) (v2:uvalue), P v1 -> P v2 -> P (UVALUE_IBinop iop v1 v2).
-    Hypothesis IH_ICmp           : forall (cmp:icmp)   (v1:uvalue) (v2:uvalue), P v1 -> P v2 -> P (UVALUE_ICmp cmp v1 v2).
-    Hypothesis IH_FBinop         : forall (fop:fbinop) (fm:list fast_math) (v1:uvalue) (v2:uvalue), P v1 -> P v2 -> P (UVALUE_FBinop fop fm v1 v2).
-    Hypothesis IH_FCmp           : forall (cmp:fcmp)   (v1:uvalue) (v2:uvalue), P v1 -> P v2 -> P (UVALUE_FCmp cmp v1 v2).
-    Hypothesis IH_Conversion     : forall (conv:conversion_type) (t_from:dtyp) (v:uvalue) (t_to:dtyp), P v -> P (UVALUE_Conversion conv t_from v t_to).
-    Hypothesis IH_GetElementPtr  : forall (t:dtyp) (ptrval:uvalue) (idxs:list (uvalue)), P ptrval -> (forall idx, InT idx idxs -> P idx) -> P (UVALUE_GetElementPtr t ptrval idxs).
-    Hypothesis IH_ExtractElement : forall (t:dtyp) (vec: uvalue) (idx: uvalue), P vec -> P idx -> P (UVALUE_ExtractElement t vec idx).
-    Hypothesis IH_InsertElement  : forall (t:dtyp) (vec: uvalue) (elt:uvalue) (idx:uvalue), P vec -> P elt -> P idx -> P (UVALUE_InsertElement t vec elt idx).
-    Hypothesis IH_ShuffleVector  : forall (t:dtyp) (vec1:uvalue) (vec2:uvalue) (idxmask:uvalue), P vec1 -> P vec2 -> P idxmask -> P (UVALUE_ShuffleVector t vec1 vec2 idxmask).
-    Hypothesis IH_ExtractValue   : forall (t:dtyp) (vec:uvalue) (idxs:list LLVMAst.int), P vec -> P (UVALUE_ExtractValue t vec idxs).
-    Hypothesis IH_InsertValue    : forall (t:dtyp) (vec:uvalue) (et:dtyp) (elt:uvalue) (idxs:list LLVMAst.int), P vec -> P elt -> P (UVALUE_InsertValue t vec et elt idxs).
-    Hypothesis IH_Select         : forall (cnd:uvalue) (v1:uvalue) (v2:uvalue), P cnd -> P v1 -> P v2 -> P (UVALUE_Select cnd v1 v2).
-    Hypothesis IH_ExtractByte : forall (uv : uvalue) (dt : dtyp) (idx : uvalue) (sid : N), P uv -> P idx -> P (UVALUE_ExtractByte uv dt idx sid).
-    Hypothesis IH_ConcatBytes : forall (dt : dtyp) (uvs : list uvalue),
-        (forall u, InT u uvs -> P u) ->
-        P (UVALUE_ConcatBytes uvs dt).
-
-    Lemma uvalue_rec' : forall (uv:uvalue), P uv.
-      fix IH 1.
-      remember P as P0 in IH.
-      destruct uv; auto; subst.
-      - revert fields.
-        fix IHfields 1. intros [|u' fields']. intros. apply IH_Struct_nil.
-        apply IH_Struct_cons.
-        apply IH.
-        apply IHfields.
-      - revert fields.
-        fix IHfields 1. intros [|u' fields']. intros. apply IH_Packed_struct_nil.
-        apply IH_Packed_struct_cons.
-        apply IH.
-        apply IHfields.
-      - revert elts.
-        fix IHelts 1. intros [|u elts']. intros. apply IH_Array_nil.
-        apply IH_Array_cons.
-        apply IH.
-        apply IHelts.
-      - revert elts.
-        fix IHelts 1. intros [|u elts']. intros. apply IH_Vector_nil.
-        apply IH_Vector_cons.
-        apply IH.
-        apply IHelts.
-      - apply IH_IBinop; auto.
-      - apply IH_ICmp; auto.
-      - apply IH_FBinop; auto.
-      - apply IH_FCmp; auto.
-      - apply IH_Conversion; auto.
-      - apply IH_GetElementPtr. apply IH.
-        { revert idxs.
-          fix IHidxs 1. intros [|u idxs']. intros. inversion X.
-          intros u' [<-|Hin]. apply IH. eapply IHidxs. apply Hin.
-        }
-      - apply IH_ExtractElement; auto.
-      - apply IH_InsertElement; auto.
-      - apply IH_ShuffleVector; auto.
-      - apply IH_ExtractValue; auto.
-      - apply IH_InsertValue; auto.
-      - apply IH_Select; auto.
-      - apply IH_ExtractByte; auto.
-      - apply IH_ConcatBytes.
-        { revert uvs.
-          fix IHuvs 1. intros [|u uvs']. intros. inversion X.
-          intros u' [<-|Hin]. apply IH. eapply IHuvs. apply Hin.
-        }
-    Qed.
-  End UvalueRec'.
 
   Section UvalueInd''.
     Variable P : uvalue -> Prop.
@@ -962,7 +787,7 @@ Module DVALUE(A:Vellvm.Semantics.MemoryAddress.ADDRESS)(IP:Vellvm.Semantics.Memo
     Hypothesis IH_ExtractValue   : forall (t:dtyp) (vec:uvalue) (idxs:list LLVMAst.int), P vec -> P (UVALUE_ExtractValue t vec idxs).
     Hypothesis IH_InsertValue    : forall (t:dtyp) (vec:uvalue) (et:dtyp) (elt:uvalue) (idxs:list LLVMAst.int), P vec -> P elt -> P (UVALUE_InsertValue t vec et elt idxs).
     Hypothesis IH_Select         : forall (cnd:uvalue) (v1:uvalue) (v2:uvalue), P cnd -> P v1 -> P v2 -> P (UVALUE_Select cnd v1 v2).
-    Hypothesis IH_ExtractByte : forall (uv : uvalue) (dt : dtyp) (idx : uvalue) (sid : N), P uv -> P idx -> P (UVALUE_ExtractByte uv dt idx sid).
+    Hypothesis IH_ExtractByte : forall (uv : uvalue) (dt : dtyp) (idx : N) (sid : N), P uv -> P (UVALUE_ExtractByte uv dt idx sid).
     Hypothesis IH_ConcatBytes : forall (dt : dtyp) (uvs : list uvalue),
         (forall u, In u uvs -> P u) ->
         P (UVALUE_ConcatBytes uvs dt).
@@ -1249,7 +1074,7 @@ Module DVALUE(A:Vellvm.Semantics.MemoryAddress.ADDRESS)(IP:Vellvm.Semantics.Memo
     Hypothesis IH_ExtractValue   : forall (t:dtyp) (vec:uvalue) (idxs:list LLVMAst.int), P vec -> P (UVALUE_ExtractValue t vec idxs).
     Hypothesis IH_InsertValue    : forall (t:dtyp) (vec:uvalue) (et:dtyp) (elt:uvalue) (idxs:list LLVMAst.int), P vec -> P elt -> P (UVALUE_InsertValue t vec et elt idxs).
     Hypothesis IH_Select         : forall (cnd:uvalue) (v1:uvalue) (v2:uvalue), P cnd -> P v1 -> P v2 -> P (UVALUE_Select cnd v1 v2).
-    Hypothesis IH_ExtractByte : forall (uv : uvalue) (dt : dtyp) (idx : uvalue) (sid : N), P uv -> P idx -> P (UVALUE_ExtractByte uv dt idx sid).
+    Hypothesis IH_ExtractByte : forall (uv : uvalue) (dt : dtyp) (idx : N) (sid : N), P uv -> P (UVALUE_ExtractByte uv dt idx sid).
     Hypothesis IH_ConcatBytes : forall (dt : dtyp) (uvs : list uvalue),
         (forall u, InT u uvs -> P u) ->
         P (UVALUE_ConcatBytes uvs dt).
@@ -1995,7 +1820,7 @@ Module DVALUE(A:Vellvm.Semantics.MemoryAddress.ADDRESS)(IP:Vellvm.Semantics.Memo
         destruct (f v v')...
         destruct (f w w')...
       - destruct (f uv uv')...
-        destruct (f idx idx')...
+        destruct (N.eq_dec idx idx')...
         destruct (N.eq_dec sid sid')...
         destruct (dtyp_eq_dec dt dt')...
       - destruct (lsteq_dec uvs uvs')...
